aeneas-lean/Tree/Rebase/Soundness.lean
@@ -83,7 +83,8 @@ def Tree.RebaseEqualitySound {T : Type} (inst : core.cmp.PartialEq T T) : Tree T
       left.values.val.length = right.values.val.length →
       ∀ pair ∈ left.values.val.zip right.values.val,
         inst.ne pair.1 pair.2 = ok false → pair.1 = pair.2
-  | .Node _ left right, .Node _ baseLeft baseRight =>
+  | .Node hash left right, .Node baseHash baseLeft baseRight =>
+      triomphe.arc.Arc.ptr_eq (.Node hash left right : Tree T) (.Node baseHash baseLeft baseRight) = ok false →
       left.RebaseEqualitySound inst baseLeft ∧ right.RebaseEqualitySound inst baseRight
   | _, _ => True
 
@@ -103,6 +104,6 @@ theorem Tree.rebaseEqualitySound_of_sound {T : Type} (inst : core.cmp.PartialEq 
   | Zero depth => cases base <;> trivial
   | Node hash left right ihleft ihright =>
     cases base <;> simp only [Tree.RebaseEqualitySound]
-    exact ⟨ihleft _, ihright _⟩
+    exact fun _ => ⟨ihleft _, ihright _⟩
 
 end milhouse.tree
