aeneas-lean/Tree.lean
@@ -178,3 +178,4 @@ import Tree.BulkUpdate.Arithmetic
 import Tree.BulkUpdate.Success
 import Tree.BulkUpdate.Contents
 import Tree.ProgressiveTree.Rebase.Soundness
+import Tree.ProgressiveList.Rebase.Pointer
